ag32/ag32AddAcceleratorScript.sml
@@ -2,30 +2,80 @@ open hardwarePreamble;
 
 open arithmeticTheory;
 
-open ag32Theory ag32MachineTheory;
+open translatorTheory ag32Theory ag32MachineTheory;
 
 val _ = new_theory "ag32AddAccelerator";
 
-guess_lengths ();
-prefer_num ();
+(*val _ = guess_lengths ();
+val _ = prefer_num ();
 
-(* Accelerator that just does integer addition inefficiently *)
+(** Machine definition -- example accelerator that just does integer addition inefficiently **)
 
-val addacc_next_def = Define `
- addacc_next s =
-  if s.acc_arg_ready then
-    s with <| acc_state := 0w; acc_res_ready := F |>
+Definition addacc_next_def:
+ addacc_next (fext:ext) (s:state_circuit) (s':state_circuit) =
+  if s'.acc_arg_ready then
+    s' with <| acc_state := 0w; acc_res_ready := F |>
   else
-   case s.acc_state of
-      0w => s with acc_state := 1w
-(*  | 1w => s with acc_state := 2w *)
-    | 1w => s with <| acc_res_ready := T;
-                      acc_res := w2w ((31 >< 16) s.acc_arg + (15 >< 0) s.acc_arg) |>
-    | _ => s`;
+   case s'.acc_state of
+      0w => s' with acc_state := 1w
+(*  | 1w => s' with acc_state := 2w *)
+    | 1w => s' with <| acc_res_ready := T;
+                       acc_res := w2w ((31 >< 16) s'.acc_arg + (15 >< 0) s'.acc_arg) |>
+    | _ => s'
+End
 
-val addacc_next_next = Q.prove(
- `!init fext n.
-   let c = circuit addacc_next init fext in
+Definition ag32_def:
+ ag32 = ag32_facc addacc_next
+End
+
+Theorem ag32_trans:
+ ag32 = mk_module (procs [cpu_Next; addacc_next]) (procs []) ag32_init
+Proof
+ simp [ag32_def, ag32_facc_def]
+QED
+
+(** Is accelerator **)
+
+Triviality execute_instruction_const:
+ (execute_instruction wV aV bV PC_next fext s).acc_state = s.acc_state
+Proof
+ rw [execute_instruction_def, shift_def] \\ WORD_DECIDE_TAC
+QED
+
+Triviality decode_instruction_const:
+ (decode_instruction s).acc_state = s.acc_state ∧
+ (decode_instruction s).acc_arg_ready = s.acc_arg_ready
+Proof
+ rw [decode_instruction_def]
+QED
+
+Triviality lt_16:
+ ∀n. n < 16 ⇔ n = 0 ∨ n = 1 ∨ n = 2 ∨ n = 3 ∨ n = 4 ∨ n = 5 ∨ n = 6 ∨ n = 7 ∨ n = 8 ∨ n = 9 ∨ n = 10 ∨ n = 11 ∨ n = 12 ∨ n = 13 ∨ n = 14 ∨ n = 15
+Proof
+ ntac 8 (Cases_on ‘n’ >- simp [] \\ Cases_on ‘n'’ >- simp []) \\ simp []
+QED
+
+Triviality ALU_const:
+ ∀args s. (ALU args s).acc_state = s.acc_state ∧
+          (ALU args s).acc_arg_ready = s.acc_arg_ready
+Proof
+ PairCases \\ gen_tac \\ Cases_on ‘args0’ \\ fs [] \\
+ pop_assum (strip_assume_tac o REWRITE_RULE [lt_16]) \\
+ simp [ALU_def]
+QED
+
+Theorem cpu_Next_const:
+ (cpu_Next fext s s').acc_state = s'.acc_state
+Proof
+ rw [cpu_Next_def,
+     cpu_Next_0w_def, execute_instruction_const, decode_instruction_const, ALU_const,
+     cpu_Next_1w_def, delay_write_Next_def,
+     cpu_Next_2w_def, cpu_Next_3w_def, cpu_Next_4w_def]
+QED
+
+Triviality addacc_next_next:
+  !fext fbits n.
+   let c = ag32 fext fbits in
    if (c n).acc_arg_ready then
     (c (SUC n)).acc_state = 0w /\
     ~(c (SUC n)).acc_res_ready
@@ -38,13 +88,19 @@ val addacc_next_next = Q.prove(
        (c (SUC n)).acc_state = (c n).acc_state /\
        (c (SUC n)).acc_res_ready /\
        (c (SUC n)).acc_res = accelerator_f (c n).acc_arg
-    | _ => T`,
- rw [circuit_def, addacc_next_def, accelerator_f_def])
- |> SIMP_RULE bool_ss [LET_THM];
+    | _ => T
+Proof
+ rw [ag32_def, ag32_facc_def, mk_module_def, mk_circuit_def, procs_def,
+     addacc_next_def, cpu_Next_const] \\ gvs []
 
-val is_acc_addacc = Q.store_thm("is_acc_addacc",
- `!init fext.
-   is_acc accelerator_f (circuit addacc_next init fext)`,
+           , ,  accelerator_f_def]
+QED
+
+val addacc_next_next = addacc_next_next |> SIMP_RULE bool_ss [LET_THM];
+
+Theorem is_acc_addacc:
+ !fext fbits. is_acc accelerator_f (ag32 fext fbits)
+Proof
  rpt strip_tac \\ simp [is_acc_def] \\ qexists_tac `2` \\ gen_tac \\ strip_tac \\
  qspecl_then [`init`, `fext`] assume_tac addacc_next_next \\
 
@@ -57,6 +113,7 @@ val is_acc_addacc = Q.store_thm("is_acc_addacc",
  >- (fs [DECIDE ``!l. l < 2 <=> l = 0 \/ l = 1``] \\ rveq \\ first_x_assum (qspec_then `1` mp_tac) \\
     simp [] \\ strip_tac \\ fs [])
 
- \\ first_assum (qspec_then `0` assume_tac) \\ first_x_assum (qspec_then `1` assume_tac) \\ fs [] \\ rfs []);
+ \\ first_assum (qspec_then `0` assume_tac) \\ first_x_assum (qspec_then `1` assume_tac) \\ fs [] \\ rfs []
+QED*)
 
 val _ = export_theory ();
